Consistent naming.

lib/adts/map.bpl
@@ -1,73 +1,75 @@
-// ---------- Axioms of the map ADT
+/**
+ * The key-value map ADT.
+ */
 
 const unique get, put, contains: Method;
 
-function invoc_k(n: Invoc) : int;
-function invoc_v(n: Invoc) : int;
+function Map.key(n: Invoc): int;
+function Map.value(n: Invoc): int;
 
-axiom (forall n: Invoc :: Invoc.name(n) == put ==> invoc_k(n) == Invoc.args(n)[0]);
-axiom (forall n: Invoc :: Invoc.name(n) == put ==> invoc_v(n) == Invoc.args(n)[1]);
-axiom (forall n: Invoc :: Invoc.name(n) == get ==> invoc_k(n) == Invoc.args(n)[0]);
-axiom (forall n: Invoc :: Invoc.name(n) == contains ==> invoc_v(n) == Invoc.args(n)[0]);
+axiom (forall n: Invoc :: Invoc.name(n) == put ==> Map.key(n) == Invoc.args(n)[0]);
+axiom (forall n: Invoc :: Invoc.name(n) == put ==> Map.value(n) == Invoc.args(n)[1]);
+axiom (forall n: Invoc :: Invoc.name(n) == get ==> Map.key(n) == Invoc.args(n)[0]);
+axiom (forall n: Invoc :: Invoc.name(n) == contains ==> Map.value(n) == Invoc.args(n)[0]);
 
-// A function to restrict a SetInvoc to invocations involving key k
-function restr(s: SetInvoc, k: int) returns (t: SetInvoc);
+// A function to restrict a Set to invocations involving key ke
+function restr(s: Set, k: int) returns (t: Set);
 
 // restr is a subset
-axiom (forall s: SetInvoc, k: int :: Set_subset(restr(s, k), s));
+axiom (forall s: Set, k: int :: Set.subset(restr(s, k), s));
 
 // restr is monotonic w.r.t subset
-axiom (forall s, t: SetInvoc, k: int :: Set_subset(s, t) ==> Set_subset(restr(s, k), restr(t, k)));
+axiom (forall s, t: Set, k: int :: Set.subset(s, t) ==> Set.subset(restr(s, k), restr(t, k)));
 
 // Adding an invocation on k increases restr
-axiom (forall q: SeqInvoc, n: Invoc :: {restr(Set_ofSeq(Seq_append(q, n)), invoc_k(n))}
-        restr(Set_ofSeq(Seq_append(q, n)), invoc_k(n))
-          == Set_add(restr(Set_ofSeq(q), invoc_k(n)), n));
+axiom (forall q: Seq, n: Invoc :: {restr(Set.ofSeq(Seq.append(q, n)), Map.key(n))}
+        restr(Set.ofSeq(Seq.append(q, n)), Map.key(n))
+          == Set.add(restr(Set.ofSeq(q), Map.key(n)), n));
 
 // Adding invocations not on k preserves restr
-axiom (forall q: SeqInvoc, n: Invoc, k: int :: invoc_k(n) != k
-       ==> restr(Set_ofSeq(Seq_append(q, n)), k) == restr(Set_ofSeq(q), k));
+axiom (forall q: Seq, n: Invoc, k: int :: Map.key(n) != k
+       ==> restr(Set.ofSeq(Seq.append(q, n)), k) == restr(Set.ofSeq(q), k));
 
 type AbsState = [int]int; // Abstract state
 
 // A function to calculate the abstract state after executing a subset vis of
 // a sequence of invocations lin
-function state(vis: SetInvoc, lin: SeqInvoc) returns (m: AbsState);
+function state(vis: Set, lin: Seq) returns (m: AbsState);
 
 
 // The effect of appending an invocation on key k on state of k
-axiom (forall s1, s2: SetInvoc, q1, q2: SeqInvoc, n: Invoc ::
-       q2 == Seq_append(q1, n) && s2 == Set_add(s1, n)
-       ==> (Invoc.name(n) == put ==> state(s2, q2)[invoc_k(n)] == invoc_v(n)));
+axiom (forall s1, s2: Set, q1, q2: Seq, n: Invoc ::
+       q2 == Seq.append(q1, n) && s2 == Set.add(s1, n)
+       ==> (Invoc.name(n) == put ==> state(s2, q2)[Map.key(n)] == Map.value(n)));
 
 // Appending a get/contains invocation does not change state
-axiom (forall s1, s2: SetInvoc, q1, q2: SeqInvoc, n: Invoc, k: int ::
-       q2 == Seq_append(q1, n) && s2 == Set_add(s1, n)
+axiom (forall s1, s2: Set, q1, q2: Seq, n: Invoc, k: int ::
+       q2 == Seq.append(q1, n) && s2 == Set.add(s1, n)
        && (Invoc.name(n) == get || Invoc.name(n) == contains)
        ==> state(s2, q2)[k] == state(s1, q1)[k]);
 
 // The effect of appending an invocation on key k on state with unchanged vis
-axiom (forall s: SetInvoc, q1: SeqInvoc, n: Invoc, k: int ::
-          state(s, q1)[k] == state(s, Seq_append(q1, n))[k]);
+axiom (forall s: Set, q1: Seq, n: Invoc, k: int ::
+          state(s, q1)[k] == state(s, Seq.append(q1, n))[k]);
 
 
 // The mapping of key k depends only invocations involving k
-axiom (forall s: SetInvoc, q: SeqInvoc, k: int ::
+axiom (forall s: Set, q: Seq, k: int ::
         state(s, q)[k] == state(restr(s, k), q)[k]);
-axiom (forall q: SeqInvoc, k: int ::
-        state(Set_ofSeq(q), q)[k] == state(restr(Set_ofSeq(q), k), q)[k]);
+axiom (forall q: Seq, k: int ::
+        state(Set.ofSeq(q), q)[k] == state(restr(Set.ofSeq(q), k), q)[k]);
 
 // Taking union with a restriction of a super-set means restrictions are same
-axiom (forall s0, s1, t: SetInvoc, k: int ::
-        s1 == Set_union(s0, t) && Set_subset(restr(s0, k), t) ==>
+axiom (forall s0, s1, t: Set, k: int ::
+        s1 == Set.union(s0, t) && Set.subset(restr(s0, k), t) ==>
           restr(s1, k) == restr(t, k)
 );
 
 // Union of disjoint keys means state comes from one of the two sets
-procedure {:layer 1} lemma_state_Set_union(k: int, K: int, s, t: SetInvoc);
-  requires (forall n: Invoc :: Set_elem(n, s) ==> invoc_k(n) < k);
-  requires (forall n: Invoc :: Set_elem(n, t) ==> k <= invoc_k(n));
+procedure {:layer 1} lemma_state_Set.union(k: int, K: int, s, t: Set);
+  requires (forall n: Invoc :: Set.elem(n, s) ==> Map.key(n) < k);
+  requires (forall n: Invoc :: Set.elem(n, t) ==> k <= Map.key(n));
   ensures (forall i: int :: 0 <= i && i < k ==>
-    state(Set_union(s, t), lin)[i] == state(s, lin)[i]);
+    state(Set.union(s, t), lin)[i] == state(s, lin)[i]);
   ensures (forall i: int :: k <= i && i < K ==>
-    state(Set_union(s, t), lin)[i] == state(t, lin)[i]);
+    state(Set.union(s, t), lin)[i] == state(t, lin)[i]);
