lib/prelude/invocations.bpl
@@ -1,9 +1,9 @@
-// ---------- Types of methods and invocations
+/**
+ * Exported declarations
+ */
 
 type Method;
-
 type Invoc;
-
 type Value = int;
 type ArgList = [int] Value;
 
@@ -11,111 +11,97 @@ function Invoc.name(i: Invoc): Method;
 function Invoc.args(i: Invoc): ArgList;
 function Invoc.rets(i: Invoc): ArgList;
 
+// Sequences of invocations
+type Seq;
+function Seq.append(s: Seq, o: Invoc): Seq;
+function Seq.elem(n: Invoc, s: Seq): bool;
+
+// Sets of invocations
+type Set;
+const Set.empty: Set;
+function Set.elem(n: Invoc, s: Set): bool;
+function Set.subset(s: Set, t: Set): bool;
+function Set.union(s1: Set, s2: Set): Set;
+function Set.unionAll(m: [int] Set, i: int, j: int): Set;
+function Set.ofSeq(q: Seq): Set;
+function Set.add(s: Set, n: Invoc): Set;
+function Set.addAll(m: [int] Set, n: Invoc, i: int, j: int): [int] Set;
+
+/**
+ * Internal declarations
+ */
+
 // Boilerplate stuff for linear variables
-function {:builtin "MapConst"} MapConstBool(bool) : [Invoc]bool;
-function {:inline} {:linear "this"} InvocCollector(x: Invoc) : [Invoc]bool
+function {:builtin "MapConst"} MapConstBool(bool): [Invoc] bool;
+function {:inline} {:linear "this"} InvocCollector(x: Invoc): [Invoc] bool
 {
   MapConstBool(false)[x := true]
 }
 
-
-// ---------- Types and axiomatization of sequences (of invocations)
-
-// Sequences of invocations
-type SeqInvoc;
-
-function Seq_append(s: SeqInvoc, o: Invoc) returns (t: SeqInvoc);
-
-function Seq_elem(n: Invoc, s: SeqInvoc) : bool;
-
 // Relationship between elem and append
-axiom (forall n1, n2: Invoc, s: SeqInvoc :: {Seq_elem(n1, Seq_append(s, n2))}
-       Seq_elem(n1, s) ==> Seq_elem(n1, Seq_append(s, n2)));
+axiom (forall n1, n2: Invoc, s: Seq :: {Seq.elem(n1, Seq.append(s, n2))}
+       Seq.elem(n1, s) ==> Seq.elem(n1, Seq.append(s, n2)));
 
-axiom (forall n: Invoc, s: SeqInvoc :: {Seq_elem(n, Seq_append(s, n))}
-       Seq_elem(n, Seq_append(s, n)));
+axiom (forall n: Invoc, s: Seq :: {Seq.elem(n, Seq.append(s, n))}
+       Seq.elem(n, Seq.append(s, n)));
 
+// Set.empty is a subset of anything
+axiom (forall s: Set :: Set.subset(Set.empty, s));
 
-// ---------- Types and axiomatization of sets (of invocations)
-
-// Sets of invocations
-type SetInvoc;
-const Set_empty: SetInvoc;
-
-function Set_elem(n: Invoc, s: SetInvoc) : bool;
-
-function Set_subset(s: SetInvoc, t: SetInvoc) : bool;
-
-// Set_empty is a subset of anything
-axiom (forall s: SetInvoc :: Set_subset(Set_empty, s));
-
-// Nothing is an elem of Set_empty
-axiom (forall n: Invoc :: !Set_elem(n, Set_empty));
+// Nothing is an elem of Set.empty
+axiom (forall n: Invoc :: !Set.elem(n, Set.empty));
 
 // subset is reflexive
-axiom (forall s: SetInvoc :: Set_subset(s, s));
+axiom (forall s: Set :: Set.subset(s, s));
 
 // subset is transitive
-axiom (forall s, t, u: SetInvoc :: Set_subset(s, t) && Set_subset(t, u) ==> Set_subset(s, u));
+axiom (forall s, t, u: Set :: Set.subset(s, t) && Set.subset(t, u) ==> Set.subset(s, u));
 
 // definition of subset in terms of elem
-axiom (forall s, t: SetInvoc :: (forall n: Invoc :: Set_elem(n, s) ==> Set_elem(n, t)) ==> Set_subset(s, t));
-
-function Set_union(s1: SetInvoc, s2: SetInvoc) returns (t: SetInvoc);
+axiom (forall s, t: Set :: (forall n: Invoc :: Set.elem(n, s) ==> Set.elem(n, t)) ==> Set.subset(s, t));
 
 // union is idempotent
-axiom (forall s: SetInvoc :: s == Set_union(s, s));
+axiom (forall s: Set :: s == Set.union(s, s));
 
 // union is associative
-axiom (forall s, t: SetInvoc :: Set_union(s, t) == Set_union(t, s));
+axiom (forall s, t: Set :: Set.union(s, t) == Set.union(t, s));
 
 // union is monotonic w.r.t subset
-axiom (forall s, t1, t2: SetInvoc :: Set_subset(t1, t2) ==> Set_subset(Set_union(s, t1), Set_union(s, t2)));
+axiom (forall s, t1, t2: Set :: Set.subset(t1, t2) ==> Set.subset(Set.union(s, t1), Set.union(s, t2)));
 
-axiom (forall s, t1, t2: SetInvoc :: Set_subset(t1, s) && Set_subset(t2, s) ==> Set_subset(Set_union(t1, t2), s));
+axiom (forall s, t1, t2: Set :: Set.subset(t1, s) && Set.subset(t2, s) ==> Set.subset(Set.union(t1, t2), s));
 
 // relation between union and elem
-axiom (forall n: Invoc, s, t: SetInvoc :: Set_elem(n, s) ==> Set_elem(n, Set_union(s, t)));
-
-// Calculate the union m[i] \cup ... \cup m[j-1]
-function unionRange(m: [int]SetInvoc, i: int, j: int) returns (s: SetInvoc);
-
-function Set_ofSeq(q: SeqInvoc) returns (s: SetInvoc);
-
-function Set_add(s: SetInvoc, n: Invoc) returns (t: SetInvoc);
+axiom (forall n: Invoc, s, t: Set :: Set.elem(n, s) ==> Set.elem(n, Set.union(s, t)));
 
 // Relation between add and elem
-axiom (forall s: SetInvoc, n1, n2: Invoc :: Set_elem(n1, Set_add(s, n2))
-       ==> n1 == n2 || Set_elem(n1, s));
-axiom (forall s: SetInvoc, n1, n2: Invoc :: Set_elem(n1, s) ==> Set_elem(n1, Set_add(s, n2)));
+axiom (forall s: Set, n1, n2: Invoc :: Set.elem(n1, Set.add(s, n2))
+       ==> n1 == n2 || Set.elem(n1, s));
+axiom (forall s: Set, n1, n2: Invoc :: Set.elem(n1, s) ==> Set.elem(n1, Set.add(s, n2)));
 
 // Relation between union and elem
-axiom (forall s, t: SetInvoc, n1: Invoc :: Set_elem(n1, Set_union(s, t))
-       ==> Set_elem(n1, s) || Set_elem(n1, t));
+axiom (forall s, t: Set, n1: Invoc :: Set.elem(n1, Set.union(s, t))
+       ==> Set.elem(n1, s) || Set.elem(n1, t));
 
 // add preserves subset relation
-axiom (forall s, t: SetInvoc, n: Invoc :: Set_subset(s, t) ==> Set_subset(Set_add(s, n), Set_add(t, n)));
-axiom (forall s, t: SetInvoc, n: Invoc :: Set_subset(s, t) ==> Set_subset(s, Set_add(t, n)));
+axiom (forall s, t: Set, n: Invoc :: Set.subset(s, t) ==> Set.subset(Set.add(s, n), Set.add(t, n)));
+axiom (forall s, t: Set, n: Invoc :: Set.subset(s, t) ==> Set.subset(s, Set.add(t, n)));
 
 // Relation between setOfSeq, add, and append
-axiom (forall q: SeqInvoc, n: Invoc :: Set_ofSeq(Seq_append(q, n)) == Set_add(Set_ofSeq(q), n));
+axiom (forall q: Seq, n: Invoc :: Set.ofSeq(Seq.append(q, n)) == Set.add(Set.ofSeq(q), n));
 
-// Relation between unionRange, add, and append
-axiom (forall t: [int]SetInvoc, i, j, k: int, q: SeqInvoc, n: Invoc ::
-        unionRange(t, i, j) == Set_ofSeq(q) && i <= k && k < j
-        ==> unionRange(t[k := Set_add(t[k], n)], i, j) == Set_ofSeq(Seq_append(q, n)));
+// Relation between unionAll, add, and append
+axiom (forall t: [int]Set, i, j, k: int, q: Seq, n: Invoc ::
+        Set.unionAll(t, i, j) == Set.ofSeq(q) && i <= k && k < j
+        ==> Set.unionAll(t[k := Set.add(t[k], n)], i, j) == Set.ofSeq(Seq.append(q, n)));
 
-// Add n to m[i], ..., m[j-1]
-function addRange(m: [int]SetInvoc, n: Invoc, i: int, j: int)
-  returns (m1: [int]SetInvoc);
+// The effect of Set.addAll
+axiom (forall m: [int]Set, n: Invoc, i: int, j: int, k: int ::
+        i <= k && k < j ==> Set.addAll(m, n, i, j)[k] == Set.add(m[k], n));
+axiom (forall m: [int]Set, n: Invoc, i: int, j: int, k: int ::
+        !(i <= k && k < j) ==> Set.addAll(m, n, i, j)[k] == m[k]);
 
-// The effect of addRange
-axiom (forall m: [int]SetInvoc, n: Invoc, i: int, j: int, k: int ::
-        i <= k && k < j ==> addRange(m, n, i, j)[k] == Set_add(m[k], n));
-axiom (forall m: [int]SetInvoc, n: Invoc, i: int, j: int, k: int ::
-        !(i <= k && k < j) ==> addRange(m, n, i, j)[k] == m[k]);
-
-// What happens to unionRange and setOfSeq when you do an addRange
-axiom (forall t: [int]SetInvoc, i, j, i1, j1: int, q: SeqInvoc, n: Invoc ::
-        unionRange(t, i, j) == Set_ofSeq(q) && i <= i1 && i1 < j1 && j1 <= j ==>
-          unionRange(addRange(t, n, i1, j1), i, j) == Set_ofSeq(Seq_append(q, n)));
+// What happens to unionAll and setOfSeq when you do an Set.addAll
+axiom (forall t: [int]Set, i, j, i1, j1: int, q: Seq, n: Invoc ::
+        Set.unionAll(t, i, j) == Set.ofSeq(q) && i <= i1 && i1 < j1 && j1 <= j ==>
+          Set.unionAll(Set.addAll(t, n, i1, j1), i, j) == Set.ofSeq(Seq.append(q, n)));
